Rename in `Raw/FlatTypeTheoryMap.v` and refactor a bit.

Raw/FlatTypeTheoryMap.v
@@ -20,116 +20,20 @@ Section FlatTypeTheoryMap.
     possibly the [Signature.map] should be extracted as a parameter,
     à la displayed categories?
   *)
-  Record TT_Map
+  Record flat_type_theory_map
     {Σ : signature σ} (T : flat_type_theory Σ)
     {Σ' : signature σ} (T' : flat_type_theory Σ')
-  := { Signature_map_of_TT_Map :> Signature.map Σ Σ'
-     ; rule_derivation_of_TT_Map
+  := { fttm_signature_map :> Signature.map Σ Σ'
+     ; fttm_rule_derivation
        : forall R : T, FlatTypeTheory.flat_rule_derivation
-                         (FlatRule.fmap Signature_map_of_TT_Map (T R))
+                         (FlatRule.fmap fttm_signature_map (T R))
                          T'
      }.
-
-  (* TODO: perhaps abstract [Family_Map_over] or something, i.e. a displayed-category version of family maps, for use in definitions like this? *)
-  Local Definition Fmap_Structural_CCs
-      {Σ Σ' : signature σ}
-      (f : Signature.map Σ Σ')
-    : Family.map
-        (Family.fmap (Closure.fmap (Judgement.fmap_judgement_total f)) (structural_rule Σ))
-        (structural_rule Σ').
-  Proof.
-    (* TODO: possible better approach:
-       - [Fmap_Family] of families commutes with sums;
-       - then use [repeat apply Fmap_Family_Sum.] or similar.  *)
-    (* TODO: intermediate approach: at least allow family map to be constructed as a single function, to avoid duplicated destructing. *)
-    apply Family.Build_map'.
-    intros [ [ [ [ c1 | ] | [c2 | c3] ] | c4 ]  | c5 ].
-    (* MANY cases here!  Really would be better with systematic way to say “in each case, apply [Fmap_Family] to the syntactic data”; perhaps something along the lines of the “judgement slots” approach? TODO: try a few by hand, then consider this. *)
-    - (* context extension *)
-      simple refine (_;_).
-      + rename c1 into ΓA.
-        refine (inl (inl (inl (Some _)))).
-        exists (Context.fmap f ΓA.1).
-        exact (Expression.fmap f ΓA.2).
-      + cbn. apply Closure.rule_eq.
-        * simple refine (Family.eq _ _). { apply idpath. }
-          cbn. intros [ [ [] | ] | ].
-          -- apply idpath.
-          -- apply (ap (fun x => (_; x))).
-             apply (ap (fun x => (_; x))).
-             apply path_forall. intros [ [] | ];
-             apply idpath.
-        * cbn. apply (ap (fun x => (_; x))).
-          apply (ap (Build_raw_context _)).
-          apply path_forall.
-          refine (plusone_rect _ _ (shape_is_extend _ _) _ _ _).
-          -- eapply concat. { refine (plusone_comp_one _ _ _ _ _ _). }
-             eapply concat. Focus 2.
-               { apply ap. refine (plusone_comp_one _ _ _ _ _ _)^. } Unfocus.
-             apply inverse. apply fmap_rename.
-          -- intros x. cbn in x.
-             eapply concat. { refine (plusone_comp_inj _ _ _ _ _ _ _). }
-             eapply concat. Focus 2.
-               { apply ap. refine (plusone_comp_inj _ _ _ _ _ _ _)^. } Unfocus.
-             apply inverse. apply fmap_rename.
-    - (* empty context *)
-      exists (inl (inl (inl None))).
-      cbn. apply Closure.rule_eq.
-      * simple refine (Family.eq _ _). { apply idpath. }
-        intros [].
-      * cbn. apply (ap (fun x => (_; x))).
-        apply (ap (Build_raw_context _)).
-        apply path_forall. refine (empty_rect _ shape_is_empty _).
-    - (* substitution *)
-      destruct c2 as [ Γ [Γ' [g [hjf hjfi]]]].
-      simple refine (_;_).
-      + refine (inl (inl (inr (inl _)))).
-        exists (Context.fmap f Γ).
-        exists (Context.fmap f Γ').
-        exists (fmap_raw_context_map f g).
-        exists hjf.
-        exact (Judgement.fmap_hypothetical_judgement f hjfi).
-      + cbn. apply Closure.rule_eq; cbn.
-        * apply inverse.
-          eapply concat. { apply Family.map_adjoin. }
-          apply ap011.
-          -- unfold Family.fmap.
-            apply ap, path_forall; intros i.
-            apply (ap (fun x => (_; x))).
-            apply (ap (fun x => (_; x))).
-            apply path_forall. intros [ [ [] | ] | ].
-            ++ refine (fmap_substitute _ _ _).
-            ++ apply idpath.
-          -- apply idpath.
-          (* Family_fmap_adjoin *)
-        * apply (ap (fun x => (_; x))). cbn.
-          apply (ap (fun x => (_; x))).
-          apply path_forall. intros i.
-          unfold Judgement.fmap_hypothetical_judgement.
-          refine (fmap_substitute _ _ _)^.
-    - (* substitution equality *)
-      destruct c3 as [ Γ [Γ' [g [g' [hjf hjfi]]]]].
-      simple refine (_;_).
-      + refine (inl (inl (inr (inr _)))).
-        exists (Context.fmap f Γ).
-        exists (Context.fmap f Γ').
-        exists (fmap_raw_context_map f g).
-        exists (fmap_raw_context_map f g').
-        exists hjf.
-        exact (Judgement.fmap_hypothetical_judgement f hjfi).
-      + admit.
-    - (* var rule *)
-      simple refine (inl (inr _) ; _); admit.
-    - (* equality rules *)
-      simple refine (inr _; _); admit.
-      (* Thest last two should be doable cleanly by the same lemmas
-      used for logical rules in [fmap] below, once that’s done. *)
-  Admitted.
 
   Local Definition fmap
     {Σ : signature σ} (T : flat_type_theory Σ)
     {Σ' : signature σ} (T' : flat_type_theory Σ')
-    (f : TT_Map T T')
+    (f : flat_type_theory_map T T')
   : Closure.map
       (Family.fmap (Closure.fmap (Judgement.fmap_judgement_total f)) (FlatTypeTheory.closure_system T))
       (FlatTypeTheory.closure_system T').
@@ -150,7 +54,7 @@ Section FlatTypeTheoryMap.
     (*   cbn in c_from_rr. rename c_from_rr into c. *)
     (*   destruct c as [i [Γ A]]. *)
     (*   unfold Derivation_of_CC; cbn. *)
-    (*   set (fc := rule_derivation_of_TT_Map _ _ f i). (* TODO: implicits! *) *)
+    (*   set (fc := fttm_rule_derivation _ _ f i). (* TODO: implicits! *) *)
     (*   set (c := T i) in *. *)
     (*   set (a := flat_rule_metas Σ c) in *. *)
     (*   unfold flat_rule_derivation in fc. cbn in fc. *)
